Proven first version of RST with selectors

pulse/ulib/LowStar.RST.fst
@@ -109,6 +109,7 @@ let is_subresource_of_intro (r0 r r1: resource) : Lemma
 let is_subresource_of_trans (r1 r2 r3: resource) : Lemma
   (requires (r1 `is_subresource_of` r2 /\ r2 `is_subresource_of` r3))
   (ensures (r1 `is_subresource_of` r3))
+  [SMTPat (r1 `is_subresource_of` r2); SMTPat (r2 `is_subresource_of` r3); SMTPat (r1 `is_subresource_of` r3)]
   =
   is_subresource_of_elim r1 r2 (r1 `is_subresource_of` r3) (fun delta12 ->
     is_subresource_of_elim r2 r3 (r1 `is_subresource_of` r3) (fun delta23 ->
@@ -123,6 +124,11 @@ let is_subresource_of_trans (r1 r2 r3: resource) : Lemma
     )
   )
 
+let is_subresource_of_refl (r: resource) : Lemma(r `is_subresource_of` r)
+  [SMTPat (r `is_subresource_of` r)]
+  =
+  assert(r `can_be_split_into` (r, empty_resource))
+
 open FStar.FunctionalExtensionality
 
 let selector r = restricted_g_t (r0:resource{r0 `is_subresource_of` r}) (fun r0 -> r0.t)
@@ -134,11 +140,12 @@ let mk_selector
 =
   on_dom_g (r0:resource{r0 `is_subresource_of` r}) (fun (r0:resource{r0 `is_subresource_of` r}) -> r0.view.sel h)
 
-let focus_selector (r: resource) (s: selector r) (r0: resource{r0 `is_subresource_of` r}) : selector r0 =
-   on_dom_g (r0':resource{r0' `is_subresource_of` r0}) (fun (r0':resource{r0' `is_subresource_of` r0}) ->
-     is_subresource_of_trans r0' r0 r;
-     s r0'
-   )
+let focus_selector (r: resource) (s: selector r) (r0: resource{r0 `is_subresource_of` r}) : s':selector r0{
+    forall (r0':resource{r0' `is_subresource_of` r0}). s' r0' == s r0'
+  } =
+  on_dom_g (r0':resource{r0' `is_subresource_of` r0}) (fun (r0':resource{r0' `is_subresource_of` r0}) ->
+    s r0'
+  )
 
 let hsprop (r: resource) : Type = selector r -> Type0
 
@@ -168,7 +175,6 @@ let hsrefine (r:resource) (p:hsprop r) : resource =
         assert(r0.view.sel h0 == r0.view.sel h1)
       in
       Classical.forall_intro aux;
-      let open FStar.FunctionalExtensionality in
       let a = r0:resource{r0 `is_subresource_of` r} in
       let b = fun r0 -> r0.t in
       extensionality_g a b sel0 sel1
@@ -181,34 +187,12 @@ let hsrefine (r:resource) (p:hsprop r) : resource =
 
 #pop-options
 
-let refine_preserves_splitting (res0 delta res1: resource) (p: hsprop res0) : Lemma
-  (res0 `can_be_split_into` (res1,delta) <==> hsrefine res0 p `can_be_split_into` (res1,delta))
-  =
-  reveal_can_be_split_into ();
-  let aux (_ : squash (res0 `can_be_split_into` (res1,delta))) : Lemma (hsrefine res0 p `can_be_split_into` (res1,delta)) =
-    admit()
-  in
-  let aux' (_ : squash (hsrefine res0 p `can_be_split_into` (res1,delta))) : Lemma (res0 `can_be_split_into` (res1,delta)) =
-    admit()
-  in
-  Classical.impl_intro aux;
-  Classical.impl_intro aux'
-
-let refine_selector (r: resource) (s:selector r) (p: hsprop r{p s}) : selector (hsrefine r p) =
-  on_dom_g (r0:resource{r0 `is_subresource_of` (hsrefine r p)}) (fun (r0:resource{r0 `is_subresource_of` (hsrefine r p)}) ->
-     is_subresource_of_elim r0 (hsrefine r p) (r0 `is_subresource_of` r) (fun delta ->
-       refine_preserves_splitting r delta r0 p
-     );
-     s r0
-   )
-
 let r_pre (res:resource) =  hsprop res
 let r_post
   (res0: resource)
-  (pre: r_pre res0)
   (a: Type)
   (res1: a -> resource) =
-  selector (hsrefine res0 pre) -> x:a -> hsprop (res1 x)
+  selector res0 -> x:a -> hsprop (res1 x)
 
 abstract
 let rst_inv (res:resource) (h:HS.mem) : GTot prop =
@@ -226,96 +210,23 @@ let rst_inv_star (res0 res1: resource) (h: HS.mem) : Lemma
   [SMTPat (rst_inv (res0 <*> res1) h)]
   = reveal_star ()
 
-// Monotonic WPs for RSTATE
-let rstate_wp (a:Type) (res0:resource) (res1:a -> resource) =
-  wp:((x:a -> imem (inv (res1 x)) -> Type0) -> imem (inv res0) -> Type0){
-      forall (p q:(x:a -> imem (inv (res1 x)) -> Type0)) h0 .
-        (forall x h1 . p x h1 ==> q x h1) ==> wp p h0 ==> wp q h0
-    }
-
-effect RSTATE (a:Type)
-              (res0:resource)                                   // Pre-resource (expected from the caller)
-              (res1:a -> resource)                              // Post-resource (returned back to the caller)
-              (wp:rstate_wp a res0 res1) =
-       STATE a
-           (fun (p:a -> HS.mem -> Type)
-              (h0:HS.mem) ->
-                inv res0 h0 /\                                  // Require the pre-resource invariant
-                rst_inv res0 h0 /\                              // Require the additional footprints invariant
-                wp (fun x h1 ->
-                     inv (res1 x) h1 /\                         // Ensure the post-resource invariant
-                     rst_inv (res1 x) h1 /\                     // Ensure the additional footprints invariant
-                     modifies res0 (res1 x) h0 h1 ==>           // Ensure that at most resources' footprints are modified
-                     p x h1) h0)                                // Prove the continuation under this hypothesis
-
-(* Pre- and postcondition style effect RST *)
-
-effect RST0
-  (a:Type)
-  (res0:resource)
-  (res1:a -> selector res0 -> resource)
-= ST a
-  (fun h0 -> res0.view.inv h0)
-  (fun h0 x h1 -> (res1 x (mk_selector res0 h0)).view.inv h1)
-
 effect RST
   (a: Type)
   (res0: resource)
   (res1: a -> resource)
   (pre: r_pre res0)
-  (post: r_post res0 pre a res1)
-= RST0
+  (post: r_post res0 a res1)
+= ST
   a
-  (hsrefine res0 pre)
-  (fun x old -> hsrefine (res1 x) (post old x))
-
-(* Bind operation for RSTATE *)
-
-let bind
-  (#a #b:Type)
-  (#res0:resource)
-  (#res1:a -> resource)
-  (#res2:b -> resource)
-  (#wp0:rstate_wp a res0 res1)
-  (#wp1:(x:a -> rstate_wp b (res1 x) res2))
-  (f:unit -> RSTATE a res0 res1 wp0)
-  (g:(x:a -> RSTATE b (res1 x) res2 (wp1 x)))
-: RSTATE b res0 res2 (fun p h0 -> wp0 (fun x h1 -> wp1 x p h1) h0) =
-  g (f ())
+  (fun h0 -> inv res0 h0 /\ rst_inv res0 h0 /\ pre (mk_selector res0 h0))
+  (fun h0 x h1 ->
+    inv (res1 x) h1 /\
+    rst_inv (res1 x) h1 /\
+    modifies res0 (res1 x) h0 h1 /\
+    post (mk_selector res0 h0) x (mk_selector (res1 x) h1)
+  )
 
 open LowStar.RST.Tactics
-
-let frame_wp
-  (#outer0:resource)
-  (#inner0:resource)
-  (#a:Type)
-  (#outer1:a -> resource)
-  (#inner1:a -> resource)
-  (delta:resource{frame_delta outer0 inner0 outer1 inner1 delta})
-  (wp:rstate_wp a inner0 inner1)
-: rstate_wp a outer0 outer1 =
-  fun p h0 ->
-    wp (fun x (h1:imem (inv (inner1 x))) ->
-      inv (outer1 x) h1 /\
-      sel (view_of delta) h0 == sel (view_of delta) h1
-      ==>
-      p x h1)
-    h0
-
-inline_for_extraction noextract let frame
-  (outer0:resource)
-  (#inner0:resource)
-  (#a:Type)
-  (outer1:a -> resource)
-  (#inner1:a -> resource)
-  (#[resolve_delta ()]
-    delta:resource{frame_delta outer0 inner0 outer1 inner1 delta})
-  (#wp:rstate_wp a inner0 inner1)
-  ($f:unit -> RSTATE a inner0 inner1 wp)
-: RSTATE a outer0 outer1 (frame_wp delta wp) =
-  reveal_view ();
-  reveal_can_be_split_into ();
-  f ()
 
 (* Generic framing operation for RST (through resource inclusion) *)
 
@@ -336,15 +247,14 @@ let frame_post
   (#inner1:a -> resource)
   (delta:resource{frame_delta outer0 inner0 outer1 inner1 delta})
   (pre:r_pre inner0)
-  (post:r_post inner0 pre a inner1)
+  (post:r_post inner0 a inner1)
   (old:selector outer0)
   (x:a)
   (modern:selector (outer1 x))
 =
   reveal_can_be_split_into ();
-  pre (focus_selector outer0 old inner0) /\
   post
-    (refine_selector inner0 (focus_selector outer0 old inner0) pre)
+    (focus_selector outer0 old inner0)
     x
     (focus_selector (outer1 x) modern (inner1 x)) /\
   old delta == modern delta
@@ -352,23 +262,40 @@ let frame_post
 
 #set-options "--no_tactics"
 
-let get (r: resource) : RST0
+let get (r: resource) : RST
   (selector r)
   (r)
-  (fun _ _ -> r)
+  (fun _ -> r)
+  (fun _ -> True)
+  (fun _ _ _ -> True)
   =
   let h = HST.get () in
   mk_selector r h
 
+#set-options "--z3rlimit 20 --max_fuel 2 --max_ifuel 2"
 
-// [DA: should be definable directly using RSTATE frame, but get
-//      an error about unexpected unification variable remaining]
+let focus_selector_equality (outer inner: resource) (h: HS.mem)
+  : Lemma
+  (requires (inv outer h /\ inner `is_subresource_of` outer))
+  (ensures (focus_selector outer (mk_selector outer h) inner == mk_selector inner h))
+  =
+  let souter = mk_selector outer h in
+  let focused = focus_selector outer souter inner in
+  let original = mk_selector inner h in
+  extensionality_g
+    (r0:resource{r0 `is_subresource_of` inner})
+    (fun r0 -> r0.t)
+    focused
+    original
+
 inline_for_extraction noextract let rst_frame
   (outer0:resource)
   (#inner0:resource)
   (#a:Type)
   (outer1:a -> resource)
   (#inner1:a -> resource)
+  (#pre:r_pre inner0)
+  (#post:r_post inner0 a inner1)
   (#[resolve_delta ()]
      delta:resource{
        FStar.Tactics.with_tactic
@@ -376,18 +303,28 @@ inline_for_extraction noextract let rst_frame
          (frame_delta outer0 inner0 outer1 inner1 delta)
      }
    )
-   (#pre:r_pre inner0)
-   (#post:r_post inner0 pre a inner1)
    ($f:unit -> RST a inner0 inner1 pre post)
 : RST a outer0 outer1
   (FStar.Tactics.by_tactic_seman resolve_frame_delta (frame_delta outer0 inner0 outer1 inner1 delta);
-    frame_pre delta pre
+     fun old ->
+       pre (focus_selector outer0 old inner0)
   )
-  (refine_preserves_splitting outer0 delta inner0 (frame_pre delta pre);
-    frame_post delta pre post)
+  (reveal_can_be_split_into ();
+    fun old x modern ->
+      post
+        (focus_selector outer0 old inner0)
+        x
+        (focus_selector (outer1 x) modern (inner1 x)) /\
+      old delta == modern delta
+  )
 =
   reveal_view ();
   reveal_can_be_split_into ();
+  reveal_rst_inv ();
   FStar.Tactics.by_tactic_seman resolve_frame_delta (frame_delta outer0 inner0 outer1 inner1 delta);
-  admit();
-  f ()
+  let h0 = HST.get () in
+  focus_selector_equality outer0 inner0 h0;
+  let x = f () in
+  let h1 = HST.get () in
+  focus_selector_equality (outer1 x) (inner1 x) h1;
+  x
